src/Translation.v
@@ -46,7 +46,7 @@ Section translate_pattern.
     | Pattern.hop pi pe pv =>
       let plan := translate_pattern' pi in
       let plan :=
-        if (In_decb (vname pv) (dom_vertices pi)) then
+        if ((PatternT.type_of Full pi (vname pv)) == (Some Value.GVertexT)) then
           Expand Into (vname (last pi)) (ename pe) (vname pv) (edir pe) plan
         else
           Expand All (vname (last pi)) (ename pe) (vname pv) (edir pe) plan
@@ -62,39 +62,26 @@ Ltac desf_translate_pvertex_pedge :=
   desf; simpls;
   normalize_bool.
 
-Theorem translate_pattern'_type pi (Hwf : Pattern.wf pi) :
+Theorem translate_pattern'_type pi (Hwf : PatternT.wfT pi) :
   type_of (translate_pattern' pi) = PatternT.type_of Full pi.
 Proof.
   all: induction pi; simpls.
   all: desf_translate_pvertex_pedge.
-  all: assert (Hwf': Pattern.wf pi) by (eauto with pattern_wf_db).
+  all: inv Hwf.
   all: extensionality n.
   all: desf_unfold_pat.
-  all: try (exfalso; eapply Pattern.wf__pv_neq_pe; now eauto).
-  all: rewrite IHpi; auto.
-  all: rewrite <- PatternT.In_dom_vertices__iff; auto.
+  all: try contradiction.
+  all: try congruence.
+  all: rewrite IHpi.
+  all: auto.
 Qed.
 
-Theorem translate_pattern_type pi (Hwf : Pattern.wf pi) :
+Theorem translate_pattern_type pi (Hwf : PatternT.wfT pi) :
   type_of (translate_pattern pi) = PatternT.type_of Explicit pi.
 Proof.
   unfold translate_pattern. simpls.
   rewrite translate_pattern'_type; auto.
   now rewrite PatternT.explicit_projT_type_of.
-Qed.
-
-Corollary translate_pattern'_type_of_GVertexT pi n (Hwf : Pattern.wf pi) :
-  (In n (Pattern.dom_vertices pi) <-> type_of (translate_pattern' pi) n = Some Value.GVertexT).
-Proof.
-  rewrite translate_pattern'_type; auto.
-  now rewrite PatternT.In_dom_vertices__iff.
-Qed.
-
-Corollary translate_pattern'_type_of_GEdgeT pi n (Hwf : Pattern.wf pi) :
-  (In n (Pattern.dom_edges pi) <-> type_of (translate_pattern' pi) n = Some Value.GEdgeT).
-Proof. 
-  rewrite translate_pattern'_type; auto.
-  now rewrite PatternT.In_dom_edges__iff.
 Qed.
 
 Theorem translate_pattern'_type_of__types pi n :
@@ -105,38 +92,32 @@ Proof.
   edestruct type_of_types as [H | [H | H]]; eauto.
 Qed.
 
-Corollary translate_pattern'__type_of_None pi n (Hwf : Pattern.wf pi)
-  (HIn_vertices : ~ In n (Pattern.dom_vertices pi))
-  (HIn_edges    : ~ In n (Pattern.dom_edges pi)) :
+Corollary translate_pattern'__type_of_None pi n (Hwf : PatternT.wfT pi)
+  (HIn_vertices : type_of (translate_pattern' pi) n <> Some Value.GVertexT)
+  (HIn_edges    : type_of (translate_pattern' pi) n <> Some Value.GEdgeT) :
     type_of (translate_pattern' pi) n = None.
 Proof.
   edestruct translate_pattern'_type_of__types as [H | [H | H]]; eauto.
-  1: eapply translate_pattern'_type_of_GVertexT in H; try eassumption.
-  2: eapply translate_pattern'_type_of_GEdgeT in H; try eassumption.
-  all: congruence.
+  all: contradiction.
 Qed.
 
-Theorem translate_pattern'_wf pi (Hwf : Pattern.wf pi) :
+Theorem translate_pattern'_wf pi (Hwf : PatternT.wfT pi) :
   ExecutionPlan.wf (translate_pattern' pi).
 Proof.
   induction pi; simpls.
-  2: assert (Pattern.wf pi) by (eapply Pattern.hop_wf; eassumption).
+  all: inv Hwf.
   all: unfold translate_pvertex, translate_pedge.
   all: desf; simpls; splits; auto.
   all: normalize_bool.
   all: desf_unfold_pat.
-  all: try apply translate_pattern'_type_of_GVertexT; try assumption.
-  all: try apply translate_pattern'_type_of_GEdgeT; try assumption.
-  all: try apply translate_pattern'__type_of_None; try assumption.
-  all: eauto with pattern_wf_db.
-
   all: try contradiction.
-  all: try intro; exfalso.
-  all: try (eapply Pattern.wf__pv_neq_pe; now eauto).
-  all: try (eapply Pattern.wf__last_neq_pe; now eauto).
+  all: try congruence.
+  all: try rewrite translate_pattern'_type; auto.
+  all: try apply PatternT.last__dom_vertices.
+  all: intros contra; eapply PatternT.last_neq_pe; eauto.
 Qed.
 
-Theorem translate_pattern_wf pi (Hwf : Pattern.wf pi) :
+Theorem translate_pattern_wf pi (Hwf : PatternT.wfT pi) :
   ExecutionPlan.wf (translate_pattern pi).
 Proof.
   unfold translate_pattern. simpls.
@@ -153,7 +134,7 @@ Module EvalQueryImpl (S : ExecutionPlan.Spec) : EvalQuery.Spec.
       EvalPlanImpl.eval graph plan.
   
   Theorem match_clause_wf graph pi
-    (Hwf_g : PropertyGraph.wf graph) (Hwf : Pattern.wf pi) :
+    (Hwf_g : PropertyGraph.wf graph) (Hwf : PatternT.wfT pi) :
       exists table', eval_match_clause graph pi = Some table'.
   Proof.
     eapply eval_wf; eauto.
@@ -162,7 +143,7 @@ Module EvalQueryImpl (S : ExecutionPlan.Spec) : EvalQuery.Spec.
 
   Theorem match_clause_type graph pi table'
     (Hres : eval_match_clause graph pi = Some table')
-    (Hwf : Pattern.wf pi) :
+    (Hwf : PatternT.wfT pi) :
       BindingTable.of_type table' (PatternT.type_of Explicit pi).
   Proof.
     unfold eval_match_clause in Hres.
@@ -203,10 +184,10 @@ Module EvalQueryImpl (S : ExecutionPlan.Spec) : EvalQuery.Spec.
       (Pattern.vname (Pattern.last pi)) (Pattern.ename pe) (Pattern.vname pv) (Pattern.edir pe).
 
   Lemma matches_hop_All graph path e v pi pe pv r'
-    (Hwf : Pattern.wf (Pattern.hop pi pe pv))
+    (Hwf : PatternT.wfT (Pattern.hop pi pe pv))
     (Htype : Rcd.type_of r' = PatternT.type_of Full (Pattern.hop pi pe pv))
     (Hmatch : Path.matches Full graph r' (Path.hop path e v) (Pattern.hop pi pe pv))
-    (HIn : ~ In (Pattern.vname pv) (Pattern.dom_vertices pi)) :
+    (HIn : PatternT.type_of Full pi (Pattern.vname pv) = None) :
       exists r, << Hexp : expansion_of_by_hop graph r' r All pi pe pv >> /\
                 << Hmatch' : Path.matches Full graph r path pi >> /\
                 << Htype' : Rcd.type_of r = PatternT.type_of Full pi >>.
@@ -221,24 +202,25 @@ Module EvalQueryImpl (S : ExecutionPlan.Spec) : EvalQuery.Spec.
       all: try extensionality k.
       all: desf_unfold_pat.
       all: try eauto using Path.matches_full_last.
-      all: try (exfalso; eapply Pattern.wf__pe_neq_last; now eauto).
-      exfalso; apply HIn. rewrite e0. apply Pattern.last__dom_vertices. }
-    { apply Path.matches_exclude. apply Path.matches_exclude.
-      all: eauto with pattern_wf_db. }
+      all: try now (exfalso; eapply PatternT.last_neq_pe; eauto).
+      all: try now (exfalso; eapply PatternT.last_neq_pv; eauto). }
+    { inv Hwf.
+      apply Path.matches_exclude. apply Path.matches_exclude.
+      all: auto. }
     { apply PatternT.matches_pattern_type_exclude_All; eauto. }
   Qed.
 
   Lemma matches_hop_Into graph path e v pi pe pv r'
-    (Hwf : Pattern.wf (Pattern.hop pi pe pv))
+    (Hwf : PatternT.wfT (Pattern.hop pi pe pv))
     (Htype : Rcd.type_of r' = PatternT.type_of Full (Pattern.hop pi pe pv))
     (Hmatch : Path.matches Full graph r' (Path.hop path e v) (Pattern.hop pi pe pv))
-    (HIn : In (Pattern.vname pv) (Pattern.dom_vertices pi)) :
+    (HIn : PatternT.type_of Full pi (Pattern.vname pv) = Some Value.GVertexT) :
       exists r, << Hexp : expansion_of_by_hop graph r' r Into pi pe pv >> /\
                 << Hmatch' : Path.matches Full graph r path pi >> /\
                 << Hdom' : Rcd.type_of r = PatternT.type_of Full pi >>.
   Proof.
     exists (Pattern.ename pe !-> None; r').
-    inv Hmatch.
+    inv Hmatch. inv Hwf.
     destruct Hpe, Hpv.
     autounfold with matches_name_db in *.
     eauto.
@@ -248,23 +230,23 @@ Module EvalQueryImpl (S : ExecutionPlan.Spec) : EvalQuery.Spec.
       
       all: try extensionality k.
       all: desf_unfold_pat.
-      all: try (exfalso; eapply Pattern.wf__pe_neq_last; now eauto).
-      all: try (exfalso; eapply Pattern.wf__pe_neq_pv; now eauto).
-      eauto using Path.matches_full_last. }
-    { apply Path.matches_exclude.
-      all: eauto with pattern_wf_db. }
+      all: try eauto using Path.matches_full_last.
+      all: try now (exfalso; eapply PatternT.last_neq_pe; eauto).
+      congruence. }
+    { apply Path.matches_exclude; auto. }
     { eapply PatternT.matches_pattern_type_exclude_Into; eauto. }
   Qed.
 
   Lemma eval_translate_pattern'_spec graph path pi table' r'
     (Hres : eval graph (translate_pattern' pi) = Some table')
-    (Hwf : Pattern.wf pi)
+    (Hwf : PatternT.wfT pi)
     (Htype : Rcd.type_of r' = PatternT.type_of Full pi)
     (Hmatch : Path.matches Full graph r' path pi) :
       In r' table'.
   Proof.
     gen_dep Htype Hres r' table' path.
     induction pi; ins.
+    all: inv Hwf.
     all: destruct path; inv Hmatch.
     all: destruct Hpv.
     all: try destruct Hpe.
@@ -291,17 +273,12 @@ Module EvalQueryImpl (S : ExecutionPlan.Spec) : EvalQuery.Spec.
             apply matches_hop_All in Hmatch; eauto
          end.
     all: desf.
-    all: match goal with
-         | [H : expand _ _ _ _ _ _ _ = _ |- _ ] =>
-            eapply expand_spec; eauto
-         end.
-    all: eapply IHpi.
-    all: eauto with pattern_wf_db.
+    all: eapply expand_spec; eauto.
   Qed.
 
   Theorem match_clause_spec graph path pi table' r'
     (Hres : eval_match_clause graph pi = Some table')
-    (Hwf : Pattern.wf pi)
+    (Hwf : PatternT.wfT pi)
     (Htype : Rcd.type_of r' = PatternT.type_of Explicit pi)
     (Hmatch : Path.matches Explicit graph r' path pi) :
       In r' table'.
@@ -315,13 +292,14 @@ Module EvalQueryImpl (S : ExecutionPlan.Spec) : EvalQuery.Spec.
 
   Lemma matches_expansion_of graph mode r r' path v_from e v_to pi pe pv
     (Hg_wf : PropertyGraph.wf graph)
-    (Hwf : Pattern.wf (Pattern.hop pi pe pv))
+    (Hwf : PatternT.wfT (Pattern.hop pi pe pv))
     (Hdom : Path.matches Full graph r path pi)
     (Hvlabel : forall l : label, Pattern.vlabel pv = Some l -> In l (vlabels graph v_to))
     (Helabel : forall l : label, Pattern.elabel pe = Some l -> elabel graph e = l)
     (Hexp : expansion_of_by_hop' graph r' r mode v_from e v_to pi pe pv) :
       Path.matches Full graph r' (Path.hop path e v_to) (Pattern.hop pi pe pv).
   Proof.
+    inv Hwf.
     apply Path.matches_cons.
     all: unfold expansion_of_by_hop', expansion_of', expansion_of in Hexp.
     all: desf; desf.
@@ -338,7 +316,7 @@ Module EvalQueryImpl (S : ExecutionPlan.Spec) : EvalQuery.Spec.
     all: subst; auto.
 
     all: desf_unfold_pat.
-    all: try (exfalso; eapply Pattern.wf__pv_neq_pe; now eauto).
+    all: try congruence.
 
     all: unfold Path.matches_direction in Hdir.
     all: desf; desf.
@@ -348,12 +326,13 @@ Module EvalQueryImpl (S : ExecutionPlan.Spec) : EvalQuery.Spec.
   Lemma eval_translate_pattern'_spec' graph pi table' r'
     (Hres : eval graph (translate_pattern' pi) = Some table')
     (Hg_wf : PropertyGraph.wf graph)
-    (Hwf : Pattern.wf pi)
+    (Hwf : PatternT.wfT pi)
     (HIn : In r' table') :
       exists path, Path.matches Full graph r' path pi.
   Proof.
     gen_dep Hres r' table'.
     induction pi; ins.
+    all: inv Hwf.
     all: desf_match_result Hres.
     all: repeat match goal with
          | [H : filter_by_label Vertices _ _ _ _ = _ |- _ ] =>
@@ -369,8 +348,7 @@ Module EvalQueryImpl (S : ExecutionPlan.Spec) : EvalQuery.Spec.
          | [H : expand _ _ _ _ _ _ _ = _ |- _ ] =>
             eapply expand_spec' in H; try eassumption; desf
          end.
-    all: try edestruct IHpi as [path ?];
-            eauto with pattern_wf_db.
+    all: try edestruct IHpi as [path ?]; eauto.
 
     all: unfold expansion_of_by_hop, expansion_of in *; desf.
     1-2: eexists (Path.start _).
@@ -391,7 +369,7 @@ Module EvalQueryImpl (S : ExecutionPlan.Spec) : EvalQuery.Spec.
   Theorem match_clause_spec' graph pi table' r'
     (Hres : eval_match_clause graph pi = Some table')
     (Hg_wf : PropertyGraph.wf graph)
-    (Hwf : Pattern.wf pi)
+    (Hwf : PatternT.wfT pi)
     (HIn : In r' table') :
       exists path, Path.matches Explicit graph r' path pi.
   Proof.
